feat: logical equivalence for modal logic (#535)
Adds logical equivalence for modal logic, proving that it is a
`Congruence` (for any modal logic, regardless of the class of models
considered) and a `LogicalEquivalence` (for logic K, i.e., when
considering the class of all models).

The PR also renames `Proposition.neg` to `Proposition.not` and adds a
useful lemma on `Proposition.iff`.

Depends on #528.

---------

Co-authored-by: Chris Henson <46805207+chenson2018@users.noreply.github.com>

Cslib/Logics/Modal/Denotation.lean
@@ -25,7 +25,7 @@ open scoped Proposition InferenceSystem
 def Proposition.denotation (m : Model World Atom) :
     Proposition Atom → Set World
   | .atom p => {w | m.v w p}
-  | .neg φ => (φ.denotation m)ᶜ
+  | .not φ => (φ.denotation m)ᶜ
   | .and φ₁ φ₂ => φ₁.denotation m ∩ φ₂.denotation m
   | .diamond φ => {w | ∃ w', m.r w w' ∧ w' ∈ φ.denotation m}
 
@@ -38,7 +38,7 @@ theorem satisfies_mem_denotation {m : Model World Atom} {φ : Proposition Atom} 
 /-- A world is in the denotation of a proposition iff it is not in the denotation of the negation
 of the proposition. -/
 @[scoped grind =]
-theorem neg_denotation {m : Model World Atom} (φ : Proposition Atom) :
+theorem not_denotation {m : Model World Atom} (φ : Proposition Atom) :
     w ∉ (¬φ).denotation m ↔ w ∈ φ.denotation m := by
   grind [_=_ satisfies_mem_denotation]
 
