Cslib.lean
@@ -139,6 +139,7 @@ public import Cslib.Logics.LinearLogic.CLL.PhaseSemantics.Basic
 public import Cslib.Logics.Modal.Basic
 public import Cslib.Logics.Modal.Cube
 public import Cslib.Logics.Modal.Denotation
+public import Cslib.Logics.Modal.LogicalEquivalence
 public import Cslib.Logics.Propositional.Defs
 public import Cslib.Logics.Propositional.NaturalDeduction.Basic
 public import Cslib.MachineLearning.PACLearning.Defs
